src/MC_algo_sandbox04.v
@@ -1,0 +1,378 @@
+Require Import MC_CTL2.
+Require Import List. Import ListNotations.
+Require Import Lia.
+
+
+Definition from_trans_to_Prop{A}(list_connections: list (A*A)): A -> A -> Prop :=
+(fun s1 s2 =>
+  let fix make_prop (list_connections: list (A*A)):Prop :=
+    match list_connections with 
+    | (b1,b2)::nil => (s1 = b1 -> (s2 = b2))
+    | (b1,b2)::tail => (s1 = b1 -> (s2 = b2)) /\ (make_prop tail)
+    | nil => False
+    end in 
+  make_prop list_connections).
+
+Definition from_label_to_Prop{A}(list_label: list (A*nat)):nat -> A -> Prop:=
+  (fun v s =>
+    let fix make_prop (list_label: list (A*nat)):Prop :=
+      match list_label with 
+      | (b,n)::nil => (s = b -> v = n)
+      | (b,n)::tail => (s = b -> v = n) /\ (make_prop tail)
+      | nil => False
+      end in 
+    make_prop list_label).
+
+Definition from_init_to_Prop{A}(list_init: list A):A->Prop :=
+(fun s =>
+  let fix make_prop (list_init: list A):Prop :=
+    match list_init with 
+    | b::nil => s = b
+    | b::tail => (s = b) \/ (make_prop tail)
+    | nil => False
+    end in 
+  make_prop list_init) 
+.
+
+
+Definition from_label_to_Prop3{A}(list_connections: list (A * (list nat))): nat -> A -> Prop :=
+(fun s1 s2 =>
+  let fix make_disjucntion_for_state_to (states_in: list nat) := 
+  match states_in with
+  | head :: nil => s1 = head
+  | head :: tail => s1 = head \/ (make_disjucntion_for_state_to tail)
+  | nil => False
+  end
+  in
+  let fix make_prop (list_connections: list (A * (list nat))):Prop :=
+    match list_connections with 
+    | (b1,b2)::nil => (s2 = b1 -> (make_disjucntion_for_state_to b2))
+    | (b1,b2)::tail => (s2 = b1 -> (make_disjucntion_for_state_to b2)) /\ (make_prop tail)
+    | nil => False
+    end in 
+  make_prop list_connections).
+  
+
+  Definition from_trans_to_Prop3{A}(list_connections: list (A * (list A))): A -> A -> Prop :=
+    (fun s1 s2 =>
+      let fix make_disjucntion_for_state_to (states_in: list A) := 
+      match states_in with
+      | head :: nil => s2 = head
+      | head :: tail => s2 = head \/ (make_disjucntion_for_state_to tail)
+      | nil => False
+      end
+      
+      in
+      let fix make_prop (list_connections: list (A * (list A))):Prop :=
+        match list_connections with 
+        | (b1,b2)::nil => (s1 = b1 -> (make_disjucntion_for_state_to b2))
+        | (b1,b2)::tail => (s1 = b1 -> (make_disjucntion_for_state_to b2)) /\ (make_prop tail)
+        | nil => False
+        end in 
+      make_prop list_connections).
+
+(* FIVE STATES *)
+Inductive   fifth : Set :=  one_fi | two_fi | three_fi | four_fi| five_fi.
+Definition  trans_fifth := from_trans_to_Prop3 [
+  (one_fi, [two_fi]);
+  (two_fi, [three_fi; four_fi]);
+  (three_fi, [four_fi]);
+  (four_fi, [five_fi]); 
+  (five_fi, [one_fi])
+].
+
+Definition  label_fifth := from_label_to_Prop3 [(one_fi, [0]); (two_fi, [0]); (three_fi, [0]); (four_fi, [0; 1; 2]); (five_fi, [0])].
+
+Definition  serial_fifth: forall w:fifth, exists (v:fifth), trans_fifth w v.
+intro; case w.
+eexists two_fi; compute; repeat split; intro; discriminate.
+eexists four_fi; compute. repeat split. intro. discriminate. intro. right. auto.
+intro; discriminate.
+intro; discriminate.
+eexists four_fi; compute. repeat split. intro. discriminate.
+intro. discriminate.
+intro. discriminate.
+intro. discriminate.
+eexists five_fi; compute. repeat split; intro; discriminate.
+eexists one_fi; compute. repeat split; intro; discriminate.
+Defined.
+
+
+Definition init_fifth := from_init_to_Prop [one_fi].
+Definition model_fifth: sts :=  {| 
+  state   := fifth; 
+  trans   := trans_fifth; 
+  init    := init_fifth; 
+  label   := label_fifth; 
+  serial  := serial_fifth 
+|}.
+
+Ltac test_ltb_m_n' m n:=
+assert (m < n);progress auto
+.
+
+Goal forall A B C:Prop, ((A->B)/\(A->C)) <->(A-> (B/\C)).
+intros.
+split.
+intros.
+destruct H.
+split.
+apply H in H0. auto.
+apply H1 in H0. auto.
+intros.
+split.
+intro. apply H in H0. destruct  H0.
+auto.
+intro.
+apply H in H0.
+destruct H0.
+auto.
+Qed.
+
+
+
+
+Ltac SOLVE_FV' init_l := (*solve satisfies model (fV ?) (?st) probleb *)
+  lazymatch type of init_l with 
+  | _ = _ =>
+    repeat split;
+    let pre := fresh "pre" in
+    intro pre; 
+    rewrite init_l in pre;
+    let rec loop_through_disj := 
+      lazymatch goal with 
+      | |- _ \/ _ => ((left; progress auto)) + (right; loop_through_disj)
+      | _ => (auto;try discriminate)
+      end
+    in
+    loop_through_disj
+  | _ => repeat split; intro ; auto
+  end
+.
+
+Theorem F2_AR: forall st: state model_fifth, 
+(init model_fifth) st -> 
+satisfies (model_fifth) (fAR (fV 0) (fV 0)) st.
+Proof.
+  let st_l := fresh "st_l" in
+  intro st_l.
+  let init_l := fresh "init_l" in
+  intro init_l. compute in init_l.
+  let path_pi := fresh "path_pi" in
+  intro path_pi.
+  let is_path_pi := fresh "is_path_pi" in
+  intro is_path_pi.
+  let first_state := fresh "first_state" in
+  intro first_state.
+  let nth_of_path := fresh "nth_of_path" in
+  intro nth_of_path.
+  left.
+
+
+Admitted.
+
+Theorem F2_IMP: forall st: state model_fifth, 
+(init model_fifth) st -> 
+satisfies (model_fifth) (fImp (fV 1) (fV 0)) st.
+Proof.
+  let st_l := fresh "st_l" in
+  intro st_l.
+  let init_l := fresh "init_l" in
+  intro init_l. compute in init_l.
+  compute.
+  intro.
+  repeat (split;try(intro; auto)).
+Defined.
+
+
+
+
+
+Inductive   square : Set :=  one_square | two_square | three_square | four_square.
+Definition  trans_square := from_trans_to_Prop3 [
+  (one_square, [two_square]);
+  (two_square, [three_square]);
+  (three_square, [four_square]);
+  (four_square, [one_square])
+].
+
+Definition  label_square := from_label_to_Prop3 [
+  (one_square, [0]);
+  (two_square, [0]); 
+  (three_square, [0;1;2]); 
+  (four_square, [2])].
+
+Definition  serial_square: forall w:square, exists (v:square), trans_square w v.
+intro; case w;
+[
+  eexists two_square |
+  eexists three_square |
+  eexists four_square |
+  eexists one_square 
+];repeat split;intro;discriminate.
+Defined.
+
+
+Definition init_square := from_init_to_Prop [one_square].
+Definition model_square: sts :=  {| 
+  state   := square; 
+  trans   := trans_square; 
+  init    := init_square; 
+  label   := label_square; 
+  serial  := serial_square 
+|}.
+
+
+
+Ltac SOLVE_AX2'' init_l solve_subformula1 := 
+  let next_state := fresh "next_state" in 
+  intro next_state;
+  let trans_to_new_state := fresh "trans_to_new_state" 
+  in 
+  intro trans_to_new_state;
+  compute in trans_to_new_state;
+  repeat (
+    let a := fresh "a" in
+    let b := fresh "b" in
+    destruct trans_to_new_state as (a&b);
+    ((apply a in init_l)+(apply b in init_l));
+    (
+      lazymatch type of init_l with 
+      | _ \/ _ => repeat( destruct init_l as [init_l|init_l])
+      | _ => idtac
+      end
+    ));
+solve_subformula1 init_l.
+
+
+
+
+Inductive   square' : Set :=  one_square' | two_square' | three_square' | four_square'.
+Definition  trans_square' := from_trans_to_Prop3 [
+  (one_square', [two_square']);
+  (two_square', [three_square']);
+  (three_square', [four_square']);
+  (four_square', [four_square'])
+].
+
+Definition  label_square' := from_label_to_Prop3 [
+  (one_square', [3]);
+  (two_square', [0;1]); 
+  (three_square', [1]); 
+  (four_square', [0;2;3])].
+
+Definition  serial_square': forall w:square', exists (v:square'), trans_square' w v.
+intros.
+case w.
+eexists two_square';repeat split; intro;try discriminate.
+eexists three_square';repeat split; intro;try discriminate; auto.
+eexists four_square';repeat split; intro;try discriminate; auto.
+eexists four_square';repeat split; intro;try discriminate; auto.
+Defined.
+
+
+Definition init_square' := from_init_to_Prop [one_square'].
+Definition model_square': sts :=  {| 
+  state   := square'; 
+  trans   := trans_square'; 
+  init    := init_square'; 
+  label   := label_square'; 
+  serial  := serial_square' 
+|}.
+
+Ltac contradict_fV sat_hyp init_l := 
+let rec loop H init_:= 
+  lazymatch type of H with
+  | _ /\ _ =>
+    let H1 := fresh "H1" in 
+    let H2 := fresh "H2" in
+    destruct H as (H1&H2);
+    ((apply H1 in init_; repeat destruct init_ as [init_|init_]; discriminate) +
+    (apply H2 in init_; repeat destruct init_ as [init_|init_]; discriminate) +
+    loop H2 init_)
+  | _ => (apply H in init_; repeat destruct init_ as [init_|init_]; discriminate)
+  end
+in
+loop sat_hyp init_l.
+
+
+Theorem F1_neg: 
+forall st: state model_square', 
+st = four_square' -> 
+satisfies (model_square') (fImp ((fV 1)) (fF)) st.
+Proof.
+  let st_l := fresh "st_l" in
+  intro st_l.
+  let init_l := fresh "init_l" in
+  intro init_l.
+  intro sat_hyp.
+  contradict_fV sat_hyp init_l.
+Defined.
+
+Ltac contradict_fAX model_l st_l sat_hyp init_l tac:= 
+  (* rewrite init_l in sat_hyp. *)
+  (* compute in sat_hyp. *)
+  pose proof ((serial model_l) st_l) as ser;
+  destruct ser as [v' hyp];
+  assert (hyp':=hyp);
+  (* compute in hyp. *)
+  let rec loop sat_hyp hyp hyp' init_:= 
+  lazymatch type of hyp' with
+  | _ /\ _ =>
+    let H1:= fresh "H1" in
+    let H2:= fresh "H2" in
+    destruct hyp' as (H1&H2);
+    (apply H1 in init_; repeat destruct init_ as [init_|init_];apply sat_hyp in hyp; tac hyp init_) +
+    (apply H2 in init_; repeat destruct init_ as [init_|init_];apply sat_hyp in hyp; tac hyp init_) +
+    loop sat_hyp hyp H2 init_
+  | _ => (apply hyp' in init_; repeat destruct init_ as [init_|init_];apply sat_hyp in hyp; tac hyp init_) 
+  end
+  in
+  loop sat_hyp hyp hyp' init_l.
+
+
+Theorem F1'_neg: 
+forall st: state model_square', 
+st = four_square' -> 
+satisfies (model_square') (fImp (fAX (fV 1)) (fF)) st.
+Proof.
+  let st_l := fresh "st_l" in
+  intro st_l.
+  let init_l := fresh "init_l" in
+  intro init_l.
+  intro sat_hyp.
+  contradict_fAX model_square' st_l sat_hyp init_l contradict_fV.
+Defined.
+  
+
+Theorem F1''_neg: 
+forall st: state model_square', 
+st = four_square' -> 
+satisfies (model_square') (fImp (fAX(fV 1)) (fF)) st.
+Proof.
+  let st_l := fresh "st_l" in
+  intro st_l.
+  let init_l := fresh "init_l" in
+  intro init_l.
+  intro sat_hyp.
+  compute.
+  contradict_fAX model_square' st_l sat_hyp init_l contradict_fV.
+Defined.
+
+
+
+
+Theorem F1'''_neg: 
+forall st: state model_square', 
+st = one_square' -> 
+satisfies (model_square') (fImp (fImp (fV 3)(fF)) (fF)) st.
+Proof.
+  let st_l := fresh "st_l" in
+  intro st_l.
+  let init_l := fresh "init_l" in
+  intro init_l.
+  intro sat_hyp.
+  compute in sat_hyp.
+  apply sat_hyp.
+  SOLVE_FV' init_l.
+Qed.
